Makefile
@@ -16,10 +16,10 @@ plugin: Makefile.coq
 
 install: Makefile.coq src/quickChickLib.cmx src/quickChickLib.o quickChickTool
 	$(MAKE) -f Makefile.coq install
-        # Manually copying the remaining files
-	cp src/quickChickLib.cmx $(COQLIB)/user-contrib/QuickChick
-	cp src/quickChickLib.o $(COQLIB)/user-contrib/QuickChick
-	cp src/quickChickTool $(shell echo $(PATH) | tr ':' "\n" | grep opam)/quickChick
+  # Manually copying the remaining files
+	# cp src/quickChickLib.cmx $(COQLIB)/user-contrib/QuickChick
+	# cp src/quickChickLib.o $(COQLIB)/user-contrib/QuickChick
+	# cp src/quickChickTool $(shell echo $(PATH) | tr ':' "\n" | grep opam)/quickChick
 
 quickChickTool: 
 	ocamllex  src/quickChickToolLexer.mll
